platform/Xml.v
@@ -3,11 +3,14 @@ Export XmlLang.
 
 
 Coercion XmlLang.Cdata : string >-> XmlLang.pat.
+Notation "$ x" := (XmlLang.Var x) (at level 0) : pat_scope.
 Infix "/" := XmlLang.Tag : pat_scope.
 Infix "&" := XmlLang.Both (at level 41, right associativity) : pat_scope.
+Infix ";;" := XmlLang.Ordered : pat_scope.
 Delimit Scope pat_scope with pat.
 
 Coercion XmlOutput.Cdata : string >-> XmlOutput.xml.
+Notation "$ x" := (XmlOutput.Var (x ++ "_start")%string (x ++ "_len")%string) : out_scope.
 Definition xcons (x : XmlOutput.xml) (xs : list XmlOutput.xml) : list XmlOutput.xml := x :: xs.
 Notation "<*> tag </> x1 , .. , xN </>" := (XmlOutput.Tag tag (xcons x1 .. (xcons xN nil) ..))
   (tag at level 0) : out_scope.
@@ -15,4 +18,12 @@ Delimit Scope out_scope with out.
 
 Notation "'Match' p 'Do' o 'end'" := {| Pattern := p%pat; Output := o%out |}.
 
-Ltac wf := repeat split; simpl; intuition congruence.
+Ltac wf :=
+  repeat split; repeat constructor; simpl in *; intuition (try congruence);
+    match goal with
+      | [ H : (_, _) = (_, _) |- _ ] => injection H; clear H; intros; subst
+    end;
+    match goal with
+      | [ |- context[_ = ?s] ] => solve [ exists s; intuition ]
+    end.
+
